dist/Kuiper_MatMul_Naive_Inst.cu
@@ -5,21 +5,34 @@
 __global__
 
 static void
-k_f32_rrr(size_t rows, size_t shared, size_t cols, float_t *gA, float_t *gB, float_t *gC)
+__hoisted_0(
+  size_t cols,
+  size_t cols0,
+  size_t shared,
+  size_t shared0,
+  float_t *gA,
+  size_t cols1,
+  float_t *gB,
+  size_t cols2,
+  float_t *gC
+)
 {
-  KRML_MAYBE_UNUSED_VAR(rows);
+  KRML_MAYBE_UNUSED_VAR(cols);
+  KRML_MAYBE_UNUSED_VAR(cols0);
+  KRML_MAYBE_UNUSED_VAR(shared);
+  KRML_MAYBE_UNUSED_VAR(cols1);
   size_t id = blockIdx_x();
-  size_t trow = id / cols;
-  size_t tcol = id % cols;
+  size_t trow = id / cols2;
+  size_t tcol = id % cols2;
   size_t k = (size_t)0U;
   float_t sum = (float_t)0.0f;
-  while (k < shared)
+  while (k < shared0)
   {
     size_t vk = k;
-    sum += gA[trow * shared + vk] * gB[vk * cols + tcol];
+    sum += gA[trow * shared0 + vk] * gB[vk * cols2 + tcol];
     k = vk + (size_t)1U;
   }
-  gC[trow * cols + tcol] = sum;
+  gC[trow * cols2 + tcol] = sum;
 }
 
 float_t
@@ -36,16 +49,19 @@ float_t
   float_t *gC = (float_t *)KPR_GPU_ALLOC((size_t)4U * (rows * cols));
   MUST(cudaMemcpy(gA, a, (size_t)4U * (rows * shared), cudaMemcpyHostToDevice));
   MUST(cudaMemcpy(gB, b, (size_t)4U * (shared * cols), cudaMemcpyHostToDevice));
-  KPR_KCALL(k_f32_rrr,
+  KPR_KCALL(__hoisted_0,
     rows * cols,
     (size_t)1U,
     (size_t)4U,
     (size_t)0U,
-    rows,
-    shared,
     cols,
+    cols,
+    shared,
+    shared,
     gA,
+    cols,
     gB,
+    cols,
     gC);
   cudaDeviceSynchronize();
   KRML_CHECK_SIZE(sizeof (float_t), rows * cols);
@@ -63,21 +79,34 @@ float_t
 __global__
 
 static void
-k_f64_rrr(size_t rows, size_t shared, size_t cols, double_t *gA, double_t *gB, double_t *gC)
+__hoisted_1(
+  size_t cols,
+  size_t cols0,
+  size_t shared,
+  size_t shared0,
+  double_t *gA,
+  size_t cols1,
+  double_t *gB,
+  size_t cols2,
+  double_t *gC
+)
 {
-  KRML_MAYBE_UNUSED_VAR(rows);
+  KRML_MAYBE_UNUSED_VAR(cols);
+  KRML_MAYBE_UNUSED_VAR(cols0);
+  KRML_MAYBE_UNUSED_VAR(shared);
+  KRML_MAYBE_UNUSED_VAR(cols1);
   size_t id = blockIdx_x();
-  size_t trow = id / cols;
-  size_t tcol = id % cols;
+  size_t trow = id / cols2;
+  size_t tcol = id % cols2;
   size_t k = (size_t)0U;
   double_t sum = (double_t)0.0l;
-  while (k < shared)
+  while (k < shared0)
   {
     size_t vk = k;
-    sum += gA[trow * shared + vk] * gB[vk * cols + tcol];
+    sum += gA[trow * shared0 + vk] * gB[vk * cols2 + tcol];
     k = vk + (size_t)1U;
   }
-  gC[trow * cols + tcol] = sum;
+  gC[trow * cols2 + tcol] = sum;
 }
 
 double_t
@@ -94,16 +123,19 @@ double_t
   double_t *gC = (double_t *)KPR_GPU_ALLOC((size_t)8U * (rows * cols));
   MUST(cudaMemcpy(gA, a, (size_t)8U * (rows * shared), cudaMemcpyHostToDevice));
   MUST(cudaMemcpy(gB, b, (size_t)8U * (shared * cols), cudaMemcpyHostToDevice));
-  KPR_KCALL(k_f64_rrr,
+  KPR_KCALL(__hoisted_1,
     rows * cols,
     (size_t)1U,
     (size_t)4U,
     (size_t)0U,
-    rows,
-    shared,
     cols,
+    cols,
+    shared,
+    shared,
     gA,
+    cols,
     gB,
+    cols,
     gC);
   cudaDeviceSynchronize();
   KRML_CHECK_SIZE(sizeof (double_t), rows * cols);
@@ -121,21 +153,34 @@ double_t
 __global__
 
 static void
-k_u32_rrr(size_t rows, size_t shared, size_t cols, uint32_t *gA, uint32_t *gB, uint32_t *gC)
+__hoisted_2(
+  size_t cols,
+  size_t cols0,
+  size_t shared,
+  size_t shared0,
+  uint32_t *gA,
+  size_t cols1,
+  uint32_t *gB,
+  size_t cols2,
+  uint32_t *gC
+)
 {
-  KRML_MAYBE_UNUSED_VAR(rows);
+  KRML_MAYBE_UNUSED_VAR(cols);
+  KRML_MAYBE_UNUSED_VAR(cols0);
+  KRML_MAYBE_UNUSED_VAR(shared);
+  KRML_MAYBE_UNUSED_VAR(cols1);
   size_t id = blockIdx_x();
-  size_t trow = id / cols;
-  size_t tcol = id % cols;
+  size_t trow = id / cols2;
+  size_t tcol = id % cols2;
   size_t k = (size_t)0U;
   uint32_t sum = 0U;
-  while (k < shared)
+  while (k < shared0)
   {
     size_t vk = k;
-    sum += gA[trow * shared + vk] * gB[vk * cols + tcol];
+    sum += gA[trow * shared0 + vk] * gB[vk * cols2 + tcol];
     k = vk + (size_t)1U;
   }
-  gC[trow * cols + tcol] = sum;
+  gC[trow * cols2 + tcol] = sum;
 }
 
 uint32_t
@@ -152,16 +197,19 @@ uint32_t
   uint32_t *gC = (uint32_t *)KPR_GPU_ALLOC((size_t)4U * (rows * cols));
   MUST(cudaMemcpy(gA, a, (size_t)4U * (rows * shared), cudaMemcpyHostToDevice));
   MUST(cudaMemcpy(gB, b, (size_t)4U * (shared * cols), cudaMemcpyHostToDevice));
-  KPR_KCALL(k_u32_rrr,
+  KPR_KCALL(__hoisted_2,
     rows * cols,
     (size_t)1U,
     (size_t)4U,
     (size_t)0U,
-    rows,
-    shared,
     cols,
+    cols,
+    shared,
+    shared,
     gA,
+    cols,
     gB,
+    cols,
     gC);
   cudaDeviceSynchronize();
   KRML_CHECK_SIZE(sizeof (uint32_t), rows * cols);
@@ -176,21 +224,34 @@ uint32_t
 __global__
 
 static void
-k_u64_rrr(size_t rows, size_t shared, size_t cols, uint64_t *gA, uint64_t *gB, uint64_t *gC)
+__hoisted_3(
+  size_t cols,
+  size_t cols0,
+  size_t shared,
+  size_t shared0,
+  uint64_t *gA,
+  size_t cols1,
+  uint64_t *gB,
+  size_t cols2,
+  uint64_t *gC
+)
 {
-  KRML_MAYBE_UNUSED_VAR(rows);
+  KRML_MAYBE_UNUSED_VAR(cols);
+  KRML_MAYBE_UNUSED_VAR(cols0);
+  KRML_MAYBE_UNUSED_VAR(shared);
+  KRML_MAYBE_UNUSED_VAR(cols1);
   size_t id = blockIdx_x();
-  size_t trow = id / cols;
-  size_t tcol = id % cols;
+  size_t trow = id / cols2;
+  size_t tcol = id % cols2;
   size_t k = (size_t)0U;
   uint64_t sum = 0ULL;
-  while (k < shared)
+  while (k < shared0)
   {
     size_t vk = k;
-    sum += gA[trow * shared + vk] * gB[vk * cols + tcol];
+    sum += gA[trow * shared0 + vk] * gB[vk * cols2 + tcol];
     k = vk + (size_t)1U;
   }
-  gC[trow * cols + tcol] = sum;
+  gC[trow * cols2 + tcol] = sum;
 }
 
 uint64_t
@@ -207,16 +268,19 @@ uint64_t
   uint64_t *gC = (uint64_t *)KPR_GPU_ALLOC((size_t)8U * (rows * cols));
   MUST(cudaMemcpy(gA, a, (size_t)8U * (rows * shared), cudaMemcpyHostToDevice));
   MUST(cudaMemcpy(gB, b, (size_t)8U * (shared * cols), cudaMemcpyHostToDevice));
-  KPR_KCALL(k_u64_rrr,
+  KPR_KCALL(__hoisted_3,
     rows * cols,
     (size_t)1U,
     (size_t)4U,
     (size_t)0U,
-    rows,
-    shared,
     cols,
+    cols,
+    shared,
+    shared,
     gA,
+    cols,
     gB,
+    cols,
     gC);
   cudaDeviceSynchronize();
   KRML_CHECK_SIZE(sizeof (uint64_t), rows * cols);
@@ -231,20 +295,249 @@ uint64_t
 __global__
 
 static void
-k_u64_ccc(size_t rows, size_t shared, size_t cols, uint64_t *gA, uint64_t *gB, uint64_t *gC)
+__hoisted_4(
+  size_t cols,
+  size_t cols0,
+  size_t shared,
+  size_t rows,
+  float_t *gA,
+  size_t shared0,
+  float_t *gB,
+  size_t rows0,
+  float_t *gC
+)
 {
+  KRML_MAYBE_UNUSED_VAR(cols);
+  KRML_MAYBE_UNUSED_VAR(shared);
+  KRML_MAYBE_UNUSED_VAR(rows);
   size_t id = blockIdx_x();
-  size_t trow = id / cols;
-  size_t tcol = id % cols;
+  size_t trow = id / cols0;
+  size_t tcol = id % cols0;
   size_t k = (size_t)0U;
-  uint64_t sum = 0ULL;
-  while (k < shared)
+  float_t sum = (float_t)0.0f;
+  while (k < shared0)
   {
     size_t vk = k;
-    sum += gA[vk * rows + trow] * gB[tcol * shared + vk];
+    sum += gA[vk * rows0 + trow] * gB[tcol * shared0 + vk];
     k = vk + (size_t)1U;
   }
-  gC[tcol * rows + trow] = sum;
+  gC[tcol * rows0 + trow] = sum;
+}
+
+float_t
+*Kuiper_MatMul_Naive_Inst_matmul_f32_ccc(
+  size_t rows,
+  size_t shared,
+  size_t cols,
+  float_t *a,
+  float_t *b
+)
+{
+  float_t *gA = (float_t *)KPR_GPU_ALLOC((size_t)4U * (rows * shared));
+  float_t *gB = (float_t *)KPR_GPU_ALLOC((size_t)4U * (shared * cols));
+  float_t *gC = (float_t *)KPR_GPU_ALLOC((size_t)4U * (rows * cols));
+  MUST(cudaMemcpy(gA, a, (size_t)4U * (rows * shared), cudaMemcpyHostToDevice));
+  MUST(cudaMemcpy(gB, b, (size_t)4U * (shared * cols), cudaMemcpyHostToDevice));
+  KPR_KCALL(__hoisted_4,
+    rows * cols,
+    (size_t)1U,
+    (size_t)4U,
+    (size_t)0U,
+    cols,
+    cols,
+    shared,
+    rows,
+    gA,
+    shared,
+    gB,
+    rows,
+    gC);
+  cudaDeviceSynchronize();
+  KRML_CHECK_SIZE(sizeof (float_t), rows * cols);
+  float_t *c = (float_t *)KRML_HOST_MALLOC(sizeof (float_t) * (rows * cols));
+  if (c != NULL)
+    for (uint32_t _i = 0U; _i < rows * cols; ++_i)
+      c[_i] = (float_t)0.0f;
+  MUST(cudaMemcpy(c, gC, (size_t)4U * (rows * cols), cudaMemcpyDeviceToHost));
+  MUST(cudaFree(gA));
+  MUST(cudaFree(gB));
+  MUST(cudaFree(gC));
+  return c;
+}
+
+__global__
+
+static void
+__hoisted_5(
+  size_t cols,
+  size_t cols0,
+  size_t shared,
+  size_t rows,
+  double_t *gA,
+  size_t shared0,
+  double_t *gB,
+  size_t rows0,
+  double_t *gC
+)
+{
+  KRML_MAYBE_UNUSED_VAR(cols);
+  KRML_MAYBE_UNUSED_VAR(shared);
+  KRML_MAYBE_UNUSED_VAR(rows);
+  size_t id = blockIdx_x();
+  size_t trow = id / cols0;
+  size_t tcol = id % cols0;
+  size_t k = (size_t)0U;
+  double_t sum = (double_t)0.0l;
+  while (k < shared0)
+  {
+    size_t vk = k;
+    sum += gA[vk * rows0 + trow] * gB[tcol * shared0 + vk];
+    k = vk + (size_t)1U;
+  }
+  gC[tcol * rows0 + trow] = sum;
+}
+
+double_t
+*Kuiper_MatMul_Naive_Inst_matmul_f64_ccc(
+  size_t rows,
+  size_t shared,
+  size_t cols,
+  double_t *a,
+  double_t *b
+)
+{
+  double_t *gA = (double_t *)KPR_GPU_ALLOC((size_t)8U * (rows * shared));
+  double_t *gB = (double_t *)KPR_GPU_ALLOC((size_t)8U * (shared * cols));
+  double_t *gC = (double_t *)KPR_GPU_ALLOC((size_t)8U * (rows * cols));
+  MUST(cudaMemcpy(gA, a, (size_t)8U * (rows * shared), cudaMemcpyHostToDevice));
+  MUST(cudaMemcpy(gB, b, (size_t)8U * (shared * cols), cudaMemcpyHostToDevice));
+  KPR_KCALL(__hoisted_5,
+    rows * cols,
+    (size_t)1U,
+    (size_t)4U,
+    (size_t)0U,
+    cols,
+    cols,
+    shared,
+    rows,
+    gA,
+    shared,
+    gB,
+    rows,
+    gC);
+  cudaDeviceSynchronize();
+  KRML_CHECK_SIZE(sizeof (double_t), rows * cols);
+  double_t *c = (double_t *)KRML_HOST_MALLOC(sizeof (double_t) * (rows * cols));
+  if (c != NULL)
+    for (uint32_t _i = 0U; _i < rows * cols; ++_i)
+      c[_i] = (double_t)0.0l;
+  MUST(cudaMemcpy(c, gC, (size_t)8U * (rows * cols), cudaMemcpyDeviceToHost));
+  MUST(cudaFree(gA));
+  MUST(cudaFree(gB));
+  MUST(cudaFree(gC));
+  return c;
+}
+
+__global__
+
+static void
+__hoisted_6(
+  size_t cols,
+  size_t cols0,
+  size_t shared,
+  size_t rows,
+  uint32_t *gA,
+  size_t shared0,
+  uint32_t *gB,
+  size_t rows0,
+  uint32_t *gC
+)
+{
+  KRML_MAYBE_UNUSED_VAR(cols);
+  KRML_MAYBE_UNUSED_VAR(shared);
+  KRML_MAYBE_UNUSED_VAR(rows);
+  size_t id = blockIdx_x();
+  size_t trow = id / cols0;
+  size_t tcol = id % cols0;
+  size_t k = (size_t)0U;
+  uint32_t sum = 0U;
+  while (k < shared0)
+  {
+    size_t vk = k;
+    sum += gA[vk * rows0 + trow] * gB[tcol * shared0 + vk];
+    k = vk + (size_t)1U;
+  }
+  gC[tcol * rows0 + trow] = sum;
+}
+
+uint32_t
+*Kuiper_MatMul_Naive_Inst_matmul_u32_ccc(
+  size_t rows,
+  size_t shared,
+  size_t cols,
+  uint32_t *a,
+  uint32_t *b
+)
+{
+  uint32_t *gA = (uint32_t *)KPR_GPU_ALLOC((size_t)4U * (rows * shared));
+  uint32_t *gB = (uint32_t *)KPR_GPU_ALLOC((size_t)4U * (shared * cols));
+  uint32_t *gC = (uint32_t *)KPR_GPU_ALLOC((size_t)4U * (rows * cols));
+  MUST(cudaMemcpy(gA, a, (size_t)4U * (rows * shared), cudaMemcpyHostToDevice));
+  MUST(cudaMemcpy(gB, b, (size_t)4U * (shared * cols), cudaMemcpyHostToDevice));
+  KPR_KCALL(__hoisted_6,
+    rows * cols,
+    (size_t)1U,
+    (size_t)4U,
+    (size_t)0U,
+    cols,
+    cols,
+    shared,
+    rows,
+    gA,
+    shared,
+    gB,
+    rows,
+    gC);
+  cudaDeviceSynchronize();
+  KRML_CHECK_SIZE(sizeof (uint32_t), rows * cols);
+  uint32_t *c = (uint32_t *)KRML_HOST_CALLOC(rows * cols, sizeof (uint32_t));
+  MUST(cudaMemcpy(c, gC, (size_t)4U * (rows * cols), cudaMemcpyDeviceToHost));
+  MUST(cudaFree(gA));
+  MUST(cudaFree(gB));
+  MUST(cudaFree(gC));
+  return c;
+}
+
+__global__
+
+static void
+__hoisted_7(
+  size_t cols,
+  size_t cols0,
+  size_t shared,
+  size_t rows,
+  uint64_t *gA,
+  size_t shared0,
+  uint64_t *gB,
+  size_t rows0,
+  uint64_t *gC
+)
+{
+  KRML_MAYBE_UNUSED_VAR(cols);
+  KRML_MAYBE_UNUSED_VAR(shared);
+  KRML_MAYBE_UNUSED_VAR(rows);
+  size_t id = blockIdx_x();
+  size_t trow = id / cols0;
+  size_t tcol = id % cols0;
+  size_t k = (size_t)0U;
+  uint64_t sum = 0ULL;
+  while (k < shared0)
+  {
+    size_t vk = k;
+    sum += gA[vk * rows0 + trow] * gB[tcol * shared0 + vk];
+    k = vk + (size_t)1U;
+  }
+  gC[tcol * rows0 + trow] = sum;
 }
 
 uint64_t
@@ -261,16 +554,19 @@ uint64_t
   uint64_t *gC = (uint64_t *)KPR_GPU_ALLOC((size_t)8U * (rows * cols));
   MUST(cudaMemcpy(gA, a, (size_t)8U * (rows * shared), cudaMemcpyHostToDevice));
   MUST(cudaMemcpy(gB, b, (size_t)8U * (shared * cols), cudaMemcpyHostToDevice));
-  KPR_KCALL(k_u64_ccc,
+  KPR_KCALL(__hoisted_7,
     rows * cols,
     (size_t)1U,
     (size_t)4U,
     (size_t)0U,
-    rows,
-    shared,
     cols,
+    cols,
+    shared,
+    rows,
     gA,
+    shared,
     gB,
+    rows,
     gC);
   cudaDeviceSynchronize();
   KRML_CHECK_SIZE(sizeof (uint64_t), rows * cols);
