src/lib/poly/Kuiper.MatMul.Naive.fsti
@@ -8,41 +8,16 @@ to do the computation. *)
 open Kuiper
 open Kuiper.MatMulGPU.Type
 open Kuiper.Matrix.Reprs.Type
-module SZ = FStar.SizeT
-
-inline_for_extraction
-val kernel_fixed_ty
-  (et : Type0) {| scalar et |}
-  (#rows #shared #cols : nat)
-  (lA : mlayout rows shared)
-  (lB : mlayout shared cols)
-  (lC : mlayout rows cols)
-  {| clayout lA |}
-  {| clayout lB |}
-  {| clayout lC |}
-: Type0
 
 inline_for_extraction noextract
-val kernel_fixed
-  (#et : Type0) {| scalar et |}
-  (#rows #shared #cols : SZ.t)
-  (lA : mlayout rows shared)
-  (lB : mlayout shared cols)
-  (lC : mlayout rows cols)
-  {| clayout lA |}
-  {| clayout lB |}
-  {| clayout lC |}
-: kernel_fixed_ty et lA lB lC
+val matmul_gpu : matmul_gpu_ty
+  // (#et : Type0) {| scalar et |}
+  // (#rows #shared #cols : szp)
+  // (#lA : mlayout rows shared)
+  // (#lB : mlayout shared cols)
+  // (#lC : mlayout rows cols)
+  // {| clayout lA |}
+  // {| clayout lB |}
+  // {| clayout lC |}
+  // : matmul_gpu_ty_type_dims_repr et lA lB lC
 
-inline_for_extraction noextract
-val matmul_gpu_fixed
-  (#et : Type0) {| scalar et |}
-  (#rows #shared #cols : szp)
-  (#lA : mlayout rows shared)
-  (#lB : mlayout shared cols)
-  (#lC : mlayout rows cols)
-  {| clayout lA |}
-  {| clayout lB |}
-  {| clayout lC |}
-  (kk : kernel_fixed_ty et lA lB lC #_ #_ #_)
-  : matmul_gpu_ty_type_dims_repr et lA lB lC
